theories/Monad.v
@@ -10,67 +10,56 @@ From CVM Require Export Attestation_Session St IO_Axioms Utils.
 From CVM Require Import Interface.Interface.
 
 (** * CVM monadic primitive operations *)
-Create HintDb cvm.
-
 Definition get_st : CVM cvm_st :=
-  ↑cs (
-    st <- get ;;s
-    ↑sr (res st)
-  ).
+  CVM_get.
 Hint Unfold get_st : cvm.
 
 Definition get_config : CVM Session_Config :=
-  conf <- ask ;;c
-  ↑cs (
-    ↑sr (res conf)
-  ).
+  CVM_ask.
 Hint Unfold get_config : cvm.
 
 Definition get_trace : CVM (list Ev) :=
-  st <- get_st ;;;c
-  ret (st_trace st).
+  st <- get_st ;;cvm
+  CVM_ret (st_trace st).
 Hint Unfold get_trace : cvm.
 
 Definition get_evid : CVM Event_ID :=
-  st <~ get_st ;;;
-  ret (st_evid st).
+  st <- get_st ;;cvm
+  CVM_ret (st_evid st).
 Hint Unfold get_evid : cvm.
 
 Definition put_trace (tr' : list Ev) : CVM unit :=
-  i <~ get_evid ;;;
-  conf <~ get_config ;;;
-  put (mk_st tr' i, conf).
+  i <- get_evid ;;cvm
+  CVM_put (mk_st tr' i).
 Hint Unfold put_trace : cvm.
 
 Definition put_evid (i' : Event_ID) : CVM unit :=
-  tr <~ get_trace ;;;
-  conf <~ get_config ;;;
-  put (mk_st tr i', conf).
+  tr <- get_trace ;;cvm
+  CVM_put (mk_st tr i').
 Hint Unfold put_evid : cvm.
 
 Definition get_pl : CVM Plc :=
-  sc <~ get_config ;;;
-  ret (session_plc sc).
+  sc <- get_config ;;cvm
+  CVM_ret (session_plc sc).
 Hint Unfold get_pl : cvm.
 
 Definition inc_id : CVM Event_ID :=
-  tr <~ get_trace ;;;
-  i <~ get_evid ;;;
-  conf <~ get_config ;;;
-  put (mk_st tr (Nat.add i 1), conf) ;;;
-  ret i.
+  tr <- get_trace ;;cvm
+  i <- get_evid ;;cvm
+  CVM_put (mk_st tr (Nat.add i 1)) ;;cvm
+  CVM_ret i.
 Hint Unfold inc_id : cvm.
 
 Definition add_trace (tr:list Ev) : CVM unit :=
-  tr' <~ get_trace ;;;
+  tr' <- get_trace ;;cvm
   put_trace (tr' ++ tr).
 Hint Unfold add_trace : cvm.
 
 (* TODO: consider removing split/join events from reference semantics.
          Would make this (no-op) helper unecessary. *)
 Definition split_ev : CVM unit :=
-  p <~ get_pl ;;;
-  i <~ inc_id ;;;
+  p <- get_pl ;;cvm
+  i <- inc_id ;;cvm
   add_trace [Term_Defs.split i p].
 Hint Unfold split_ev : cvm.
 
@@ -80,44 +69,44 @@ Hint Unfold split_ev : cvm.
    CVM internal trace.  Returns the new Event_ID (used to represent raw 
    EvidenceT, relevant for appraisal verification).  *)
 Definition tag_ASP (params :ASP_PARAMS) (mpl:Plc) (e:Evidence) : CVM Event_ID :=
-  x <~ inc_id ;;;
-  add_trace [umeas x mpl params (get_et e)] ;;;
-  ret x.
+  x <- inc_id ;;cvm
+  add_trace [umeas x mpl params (get_et e)] ;;cvm
+  CVM_ret x.
 Hint Unfold tag_ASP : cvm.
 
 Local Open Scope list_scope.
 
 Definition join_seq (e1:Evidence) (e2:Evidence): CVM Evidence :=
-  p <~ get_pl ;;;
-  n <~ inc_id ;;;
+  p <- get_pl ;;cvm
+  n <- inc_id ;;cvm
   let '(evc bits1 et1) := e1 in
   let '(evc bits2 et2) := e2 in
-  add_trace [join n p] ;;;
-  ret (evc (bits1 ++ bits2) (split_evt et1 et2)).
+  add_trace [join n p] ;;cvm
+  CVM_ret (evc (bits1 ++ bits2) (split_evt et1 et2)).
 Hint Unfold join_seq : cvm.
 
 Definition hoist_result {A : Type} (r : Result A string) : CVM A :=
   match r with
-  | res a => ret a
-  | err e => fail (dispatch_error (Runtime e))
+  | res a => CVM_ret a
+  | err e => CVM_fail (dispatch_error (Runtime e))
   end.
 Hint Unfold hoist_result : cvm.
 
 Definition hoist_option {A : Type} (o : option A) (msg : string) : CVM A :=
   match o with
-  | Some a => ret a
-  | None => fail (dispatch_error (Runtime msg))
+  | Some a => CVM_ret a
+  | None => CVM_fail (dispatch_error (Runtime msg))
   end.
 Hint Unfold hoist_option : cvm.
 
 Definition get_asp_type `{DecEq ASP_ID} (a : ASP_ID) : CVM EvSig :=
-  sc <~ get_config ;;;
+  sc <- get_config ;;cvm
   let G := session_context sc in
   hoist_option ((asp_types G) ![ a ]) err_str_asp_no_type_sig.
 Hint Unfold get_asp_type : cvm.
 
 Definition get_asp_dual `{DecEq ASP_ID} (a : ASP_ID) : CVM ASP_ID :=
-  sc <~ get_config ;;;
+  sc <- get_config ;;cvm
   let G := session_context sc in
   hoist_option ((asp_comps G) ![ a ]) err_str_asp_no_compat_appr_asp.
 Hint Unfold get_asp_dual : cvm.
@@ -125,7 +114,7 @@ Hint Unfold get_asp_dual : cvm.
 Definition bundle_asp `{DecEq nat, DecEq ASP_ID} (p:Plc) (rwev : RawEv) 
     (cur_ev : Evidence) (ps:ASP_PARAMS) : CVM Evidence :=
   let '(asp_paramsC asp_id args targ_plc targ) := ps in
-  '(ev_arrow fwd in_sig out_sig) <~ get_asp_type asp_id ;;;
+  '(ev_arrow fwd in_sig out_sig) <- get_asp_type asp_id ;;cvm
   match out_sig with
   | (OutN n) =>
     match (dec_eq (List.length rwev) n) with
@@ -134,44 +123,44 @@ Definition bundle_asp `{DecEq nat, DecEq ASP_ID} (p:Plc) (rwev : RawEv)
 (* The semantics for a "REPLACE" asp are it CONSUMES all incoming evidence,
 then returns a new collection of evidence that will REPLACE the CVMs current 
 Evidence *)
-      | REPLACE => ret (evc rwev (asp_evt p ps (get_et cur_ev)))
+      | REPLACE => CVM_ret (evc rwev (asp_evt p ps (get_et cur_ev)))
 (* The semantics for a "WRAP" asp are the exact same as "REPLACE" for the 
 attestation and bundling side of the CVM. Wraps main distinction lies in the
 fact that its is a GUARANTEE, that the dual appraisal ASP is actually an
 inverse, thus allowing WRAPPED evidence to be recovered via appraisal *)
-      | WRAP => ret (evc rwev (asp_evt p ps (get_et cur_ev)))
-      | UNWRAP => fail (dispatch_error (Runtime err_str_unwrap_must_have_outwrap))
+      | WRAP => CVM_ret (evc rwev (asp_evt p ps (get_et cur_ev)))
+      | UNWRAP => CVM_fail (dispatch_error (Runtime err_str_unwrap_must_have_outwrap))
 (* The semantics for an "EXTEND" asp are it APPENDS all incoming evidence to the
 current CVM evidence bundle *)
       | EXTEND =>
         match cur_ev with
-        | evc bits et => ret (evc (rwev ++ bits) (asp_evt p ps et))
+        | evc bits et => CVM_ret (evc (rwev ++ bits) (asp_evt p ps et))
         end
       end
     | right _ => 
       (* we are not the right size, so we fail *)
-      fail (dispatch_error (Runtime errStr_raw_EvidenceT_too_long))
+      CVM_fail (dispatch_error (Runtime errStr_raw_EvidenceT_too_long))
     end
   | OutUnwrap =>
     match fwd with
-    | WRAP => fail (dispatch_error (Runtime err_str_only_unwrap_can_be_outwrap))
-    | REPLACE => fail (dispatch_error (Runtime err_str_only_unwrap_can_be_outwrap))
-    | EXTEND => fail (dispatch_error (Runtime err_str_only_unwrap_can_be_outwrap))
+    | WRAP => CVM_fail (dispatch_error (Runtime err_str_only_unwrap_can_be_outwrap))
+    | REPLACE => CVM_fail (dispatch_error (Runtime err_str_only_unwrap_can_be_outwrap))
+    | EXTEND => CVM_fail (dispatch_error (Runtime err_str_only_unwrap_can_be_outwrap))
     | UNWRAP => 
-      sc <~ get_config ;;;
+      sc <- get_config ;;cvm
       let G := (session_context sc) in
       let '(evc bits et) := cur_ev in
-      size_below_wrap' <~ hoist_result (apply_to_evidence_below G (et_size G) [Trail_UNWRAP asp_id] et) ;;;
-      size_below_wrap <~ hoist_result (size_below_wrap' ) ;;;
+      size_below_wrap' <- hoist_result (apply_to_evidence_below G (et_size G) [Trail_UNWRAP asp_id] et) ;;cvm
+      size_below_wrap <- hoist_result (size_below_wrap') ;;cvm
       (* we now need to just verify that we are the same size as what was below the wrap *)
       match (dec_eq (List.length rwev) size_below_wrap) with
-      | left _ => ret (evc rwev (asp_evt p ps et))
+      | left _ => CVM_ret (evc rwev (asp_evt p ps et))
       | right _ =>
-        fail (dispatch_error (Runtime err_str_unwrap_of_wrap_same_size))
+        CVM_fail (dispatch_error (Runtime err_str_unwrap_of_wrap_same_size))
       end
       (* match r with
       | asp_evt p' (asp_paramsC wrap_id _ _ _) et' =>
-        '(ev_arrow fwd _ _) <~ get_asp_type wrap_id ;;;
+        '(ev_arrow fwd _ _) <- get_asp_type wrap_id ;;cvm
         match fwd with
         | WRAP =>
           (* we are an UNWRAP or a WRAP, so new size is the sizer of et' *)
@@ -195,49 +184,49 @@ Hint Unfold bundle_asp : cvm.
       Extracted code should not need to use the Plc or Event_ID parameters 
       (those can be erased upon extraction). *)
 Definition do_asp (params :ASP_PARAMS) (e:RawEv) (x:Event_ID) : CVM RawEv :=
-  sc <~ get_config  ;;;
+  sc <- get_config  ;;cvm
   match (sc.(asp_cb) params e) with
-  | res r => ret r
-  | err e => fail (dispatch_error e)
+  | res r => CVM_ret r
+  | err e => CVM_fail (dispatch_error e)
   end.
 Hint Unfold do_asp : cvm.
 
 (* Simulates invoking an arbitrary ASP.  Tags the event, builds and returns 
    the new EvidenceT bundle. *)
 Definition invoke_ASP `{DecEq ASP_ID} (e : Evidence) (params : ASP_PARAMS) : CVM Evidence :=
-  p <~ get_pl ;;;
-  x <~ tag_ASP params p e ;;;
-  rawev <~ do_asp params (get_bits e) x ;;;
-  outev <~ bundle_asp p rawev e params ;;;
-  ret outev.
+  p <- get_pl ;;cvm
+  x <- tag_ASP params p e ;;cvm
+  rawev <- do_asp params (get_bits e) x ;;cvm
+  outev <- bundle_asp p rawev e params ;;cvm
+  CVM_ret outev.
 Hint Unfold invoke_ASP : cvm.
 
 (* Simulates invoking an arbitrary ASP.  Tags the event, builds and returns 
    the new EvidenceT bundle. *)
 
 Fixpoint invoke_APPR' `{DecEq ASP_ID} (r : RawEv) (et : EvidenceT) (out_evt : EvidenceT) {struct et} : CVM Evidence :=
-  sc <~ get_config ;;;
+  sc <- get_config ;;cvm
   let G := (session_context sc) in
   match et with
-  | mt_evt => ret mt_evc 
+  | mt_evt => CVM_ret mt_evc 
   | nonce_evt n' => invoke_ASP (evc r out_evt) check_nonce_params
   | asp_evt p' par et' =>
     let '(asp_paramsC asp_id args targ_plc targ) := par in
-    appr_asp_id <~ get_asp_dual asp_id ;;;
+    appr_asp_id <- get_asp_dual asp_id ;;cvm
     let dual_par := asp_paramsC appr_asp_id args targ_plc targ in
-    '(ev_arrow fwd in_sig out_sig) <~ get_asp_type asp_id ;;;
+    '(ev_arrow fwd in_sig out_sig) <- get_asp_type asp_id ;;cvm
     match fwd with
     | REPLACE => (* Only do the dual ASP *)
       invoke_ASP (evc r out_evt) dual_par
     | WRAP =>
       (* first do the dual ASP to unwrap *)
       (* NOTE: Do we need to be checking that appr_asp_id is an UNWRAP here? *)
-      '(evc r'' et'') <~ invoke_ASP (evc r out_evt) dual_par ;;;
+      '(evc r'' et'') <- invoke_ASP (evc r out_evt) dual_par ;;cvm
       (* Check that the "UNWRAP" occured properly *)
-      n' <~ hoist_result (et_size G et'') ;;;
-      n'' <~ hoist_result (et_size G et') ;;;
+      n' <- hoist_result (et_size G et'') ;;cvm
+      n'' <- hoist_result (et_size G et') ;;cvm
       match (dec_eq n' n'') with
-      | right _ => fail (dispatch_error (Runtime err_str_appr_wrap_failed))
+      | right _ => CVM_fail (dispatch_error (Runtime err_str_appr_wrap_failed))
       | left _ => (* The "UNWRAP" worked *)
         (* so do the recursive call *)
         invoke_APPR' r'' et' (asp_evt (session_plc sc) dual_par out_evt)
@@ -246,9 +235,9 @@ Fixpoint invoke_APPR' `{DecEq ASP_ID} (r : RawEv) (et : EvidenceT) (out_evt : Ev
       (* to appraise an UNWRAP is to appraise whatever is below 
       the UNWRAP and WRAP *)
       match out_sig with
-      | OutN _ => fail (dispatch_error (Runtime err_str_unwrap_must_have_outwrap)) 
+      | OutN _ => CVM_fail (dispatch_error (Runtime err_str_unwrap_must_have_outwrap)) 
       | OutUnwrap =>
-        e <~ hoist_result (apply_to_evidence_below G (fun e => invoke_APPR' r e out_evt) [Trail_UNWRAP asp_id] et') ;;;
+        e <- hoist_result (apply_to_evidence_below G (fun e => invoke_APPR' r e out_evt) [Trail_UNWRAP asp_id] et') ;;cvm
         e 
         (* e <- hoist_result (
           apply_to_asp_under_wrap G asp_id (fun e => invoke_APPR' r e out_evt) et'
@@ -258,54 +247,54 @@ Fixpoint invoke_APPR' `{DecEq ASP_ID} (r : RawEv) (et : EvidenceT) (out_evt : Ev
 
     | EXTEND =>
       match out_sig with
-      | OutUnwrap => fail (dispatch_error (Runtime err_str_extend_must_have_outn))
+      | OutUnwrap => CVM_fail (dispatch_error (Runtime err_str_extend_must_have_outn))
       | (OutN n) =>
         (* first we split, left for the appr of extended part, right for rest *)
-        split_ev ;;;
-        '(_, r_ev) <~ (hoist_result (peel_n_rawev n r)) ;;;
+        split_ev ;;cvm
+        '(_, r_ev) <- (hoist_result (peel_n_rawev n r)) ;;cvm
 
         (* on left we do the dual of EXTEND *)
-        ev1 <~ invoke_ASP (evc r out_evt) dual_par ;;;
+        ev1 <- invoke_ASP (evc r out_evt) dual_par ;;cvm
 
         (* now on right, we work only on the remaining evidence *)
         (* our new evidence is e' *)
         (* now we do the recursive call *)
-        ev2 <~ invoke_APPR' r_ev et' et' ;;;
+        ev2 <- invoke_APPR' r_ev et' et' ;;cvm
         (* now join *)
         join_seq ev1 ev2 
       end
-      (* ev' <~ invoke_ASP (asp_paramsC appr_asp_id args targ_plc targ) ;;;
+      (* ev' <- invoke_ASP (asp_paramsC appr_asp_id args targ_plc targ) ;;cvm
       put_ev ev' *)
     end
   | left_evt et' =>
-    r <~ hoist_result (apply_to_evidence_below G (fun e => invoke_APPR' r e out_evt) [Trail_LEFT] et') ;;;
+    r <- hoist_result (apply_to_evidence_below G (fun e => invoke_APPR' r e out_evt) [Trail_LEFT] et') ;;cvm
     r
 
   | right_evt et' =>
-    r <~ hoist_result (apply_to_evidence_below G (fun e => invoke_APPR' r e out_evt) [Trail_RIGHT] et') ;;;
+    r <- hoist_result (apply_to_evidence_below G (fun e => invoke_APPR' r e out_evt) [Trail_RIGHT] et') ;;cvm
     r
 
   | split_evt et1 et2 =>
-    n1 <~ hoist_result (et_size G et1) ;;;
-    n2 <~ hoist_result (et_size G et2) ;;;
-    '(ev_l, r_ev) <~ (hoist_result (peel_n_rawev n1 r)) ;;;
-    '(ev_r, rest) <~ (hoist_result (peel_n_rawev n2 r_ev)) ;;;
+    n1 <- hoist_result (et_size G et1) ;;cvm
+    n2 <- hoist_result (et_size G et2) ;;cvm
+    '(ev_l, r_ev) <- (hoist_result (peel_n_rawev n1 r)) ;;cvm
+    '(ev_r, rest) <- (hoist_result (peel_n_rawev n2 r_ev)) ;;cvm
     match rest with
     | [] => 
       if (equiv_EvidenceT G et1 (left_evt out_evt))
       then if (equiv_EvidenceT G et2 (right_evt out_evt))
       then
-        split_ev ;;; (* register event that we are splitting evidence *)
+        split_ev ;;cvm (* register event that we are splitting evidence *)
         (* first we must get out the actual Evidence for et1 *)
-        ev1 <~ invoke_APPR' ev_l et1 (left_evt out_evt) ;;;
-        ev2 <~ invoke_APPR' ev_r et2 (right_evt out_evt) ;;;
+        ev1 <- invoke_APPR' ev_l et1 (left_evt out_evt) ;;cvm
+        ev2 <- invoke_APPR' ev_r et2 (right_evt out_evt) ;;cvm
         join_seq ev1 ev2
-      else fail (dispatch_error (Runtime err_str_ev_split_failed_not_empty))
-      else fail (dispatch_error (Runtime err_str_ev_split_failed_not_empty))
-      (* ev1 <~ invoke_APPR' ev_l et1 (left_evt out_evt) ;;;
-      ev2 <~ invoke_APPR' ev_r et2 (right_evt out_evt) ;;;
+      else CVM_fail (dispatch_error (Runtime err_str_ev_split_failed_not_empty))
+      else CVM_fail (dispatch_error (Runtime err_str_ev_split_failed_not_empty))
+      (* ev1 <- invoke_APPR' ev_l et1 (left_evt out_evt) ;;cvm
+      ev2 <- invoke_APPR' ev_r et2 (right_evt out_evt) ;;cvm
       join_seq ev1 ev2 *)
-    | _ => fail (dispatch_error (Runtime err_str_ev_split_failed_not_empty))
+    | _ => CVM_fail (dispatch_error (Runtime err_str_ev_split_failed_not_empty))
     end
   end.
 
@@ -314,14 +303,14 @@ Definition invoke_APPR (e : Evidence) : CVM Evidence :=
 Hint Unfold invoke_APPR : cvm.
 
 Definition nullEv : CVM Evidence :=
-  p <~ get_pl ;;;
-  x <~ inc_id ;;;
-  add_trace [null x p] ;;;
-  ret mt_evc.
+  p <- get_pl ;;cvm
+  x <- inc_id ;;cvm
+  add_trace [null x p] ;;cvm
+  CVM_ret mt_evc.
 Hint Unfold nullEv : cvm.
 
 Definition clearEv : unit -> CVM Evidence :=
-  fun _ => ret mt_evc.
+  fun _ => CVM_ret mt_evc.
 Hint Unfold clearEv : cvm.
 
 (* Helper that interprets primitive core terms in the CVM.  *)
@@ -339,20 +328,20 @@ Hint Unfold do_prim : cvm.
 (* Monadic helper function to simulate a span of remote event IDs 
    corresponding to the size of a Term *)
 Definition inc_remote_event_ids (e : Evidence) (t:Term) : CVM unit :=
-  i <~ get_evid ;;;
-  sc <~ get_config ;;;
-  p <~ get_pl ;;;
-  n <~ hoist_result (events_size (session_context sc) p (get_et e) t) ;;;
+  i <- get_evid ;;cvm
+  sc <- get_config ;;cvm
+  p <- get_pl ;;cvm
+  n <- hoist_result (events_size (session_context sc) p (get_et e) t) ;;cvm
   put_evid (Nat.add i n).
 Hint Unfold inc_remote_event_ids : cvm.
 
 (* Monadic helper function to simulate a span of parallel event IDs 
    corresponding to the size of a Term *)
 Definition inc_par_event_ids (e : Evidence) (t: Term) : CVM unit :=
-  i <~ get_evid ;;;
-  sc <~ get_config ;;;
-  p <~ get_pl ;;;
-  n <~ hoist_result (events_size (session_context sc) p (get_et e) t) ;;;
+  i <- get_evid ;;cvm
+  sc <- get_config ;;cvm
+  p <- get_pl ;;cvm
+  n <- hoist_result (events_size (session_context sc) p (get_et e) t) ;;cvm
   put_evid (Nat.add i n).
 Hint Unfold inc_par_event_ids : cvm.
   
@@ -360,18 +349,18 @@ Hint Unfold inc_par_event_ids : cvm.
    (some rely on Admitted IO Stubs). *)
 
 Definition tag_REQ (t:Term) (p:Plc) (q:Plc) (e:Evidence) : CVM unit :=
-  reqi <~ inc_id ;;;
+  reqi <- inc_id ;;cvm
   add_trace [req reqi p q (get_et e) t].
 Hint Unfold tag_REQ : cvm.
 
 Definition tag_RPY (p:Plc) (q:Plc) (e:Evidence) : CVM unit :=
-  rpyi <~ inc_id ;;;
+  rpyi <- inc_id ;;cvm
   add_trace [rpy rpyi p q (get_et e)].
 Hint Unfold tag_RPY : cvm.
 
 Definition get_cvm_policy : CVM PolicyT := 
-  sc <~ get_config ;;;
-  ret (policy sc).
+  sc <- get_config ;;cvm
+  CVM_ret (policy sc).
 Hint Unfold get_cvm_policy : cvm.
 
 (* Remote communication primitives *)
@@ -407,68 +396,68 @@ Hint Unfold do_remote : cvm.
 
 Definition doRemote_session' (pTo:Plc) (e:Evidence) (t:Term) 
     : CVM Evidence := 
-  sc <~ get_config ;;;
+  sc <- get_config ;;cvm
   (* We need to check that the policy allows us to do this remote call *)
   match (do_remote sc pTo e t) with
-  | res e' => ret e'
-  | err s => fail s
+  | res e' => CVM_ret e'
+  | err s => CVM_fail s
   end.
 Hint Unfold doRemote_session' : cvm.
 
 Definition remote_session (p:Plc) (q:Plc) (e:Evidence) (t:Term) : CVM Evidence :=
-  tag_REQ t p q e ;;;
-  e' <~ doRemote_session' q e t ;;;
-  sc <~ get_config ;;;
-  i <~ get_evid ;;;
-  rem_evs <~ match events_fix (session_context sc) q (get_et e) t i with
-  | err e => fail (dispatch_error (Runtime e))
-  | res evs => ret evs
-  end ;;;
-  add_trace rem_evs ;;;
-  inc_remote_event_ids e t ;;;
-  ret e'.
+  tag_REQ t p q e ;;cvm
+  e' <- doRemote_session' q e t ;;cvm
+  sc <- get_config ;;cvm
+  i <- get_evid ;;cvm
+  rem_evs <- match events_fix (session_context sc) q (get_et e) t i with
+  | err e => CVM_fail (dispatch_error (Runtime e))
+  | res evs => CVM_ret evs
+  end ;;cvm
+  add_trace rem_evs ;;cvm
+  inc_remote_event_ids e t ;;cvm
+  CVM_ret e'.
 Hint Unfold remote_session : cvm.
 
 Definition doRemote (q:Plc) (e:Evidence) (t:Term) : CVM Evidence :=
-  p <~ get_pl ;;;
-  e' <~ remote_session p q e t ;;;
-  tag_RPY p q e' ;;;
-  ret e'.
+  p <- get_pl ;;cvm
+  e' <- remote_session p q e t ;;cvm
+  tag_RPY p q e' ;;cvm
+  CVM_ret e'.
 Hint Unfold doRemote : cvm.
 
 (* Primitive monadic parallel CVM thread primitives 
    (some rely on Admitted IO Stubs). *)
 
 Definition start_par_thread (e:Evidence) (t: Term) : CVM nat :=
-  p <~ get_pl ;;;
-  i <~ inc_id ;;;
+  p <- get_pl ;;cvm
+  i <- inc_id ;;cvm
   (* The loc always = the event id for the thread_start event *)
-  do_start_par_thread i e t ;;;
-  add_trace [cvm_thread_start i i p (get_et e) t] ;;;
-  ret i.
+  do_start_par_thread i e t ;;cvm
+  add_trace [cvm_thread_start i i p (get_et e) t] ;;cvm
+  CVM_ret i.
 Hint Unfold start_par_thread : cvm.
 
 Definition do_wait_par_thread (loc:Loc) (p:Plc) (e:Evidence) (t: Term) : CVM Evidence :=
   match (parallel_vm_thread loc p e t) with
-  | res e' => ret e'
-  | err s => fail s
+  | res e' => CVM_ret e'
+  | err s => CVM_fail s
   end.
 Hint Unfold do_wait_par_thread : cvm.
 
 Definition wait_par_thread (loc:Loc) (e:Evidence) (t: Term) : CVM Evidence :=
-  p <~ get_pl ;;;
-  e' <~ do_wait_par_thread loc p e t ;;;
-  i <~ get_evid ;;;
-  sc <~ get_config ;;;
-  rem_evs <~ match events_fix (session_context sc) p (get_et e) t i with
-  | err e => fail (dispatch_error (Runtime e))
-  | res evs => ret evs
-  end ;;;
-  add_trace rem_evs ;;;
-  inc_par_event_ids e t ;;;
-  i <~ inc_id ;;;
-  add_trace [cvm_thread_end i loc] ;;;
-  ret e'.
+  p <- get_pl ;;cvm
+  e' <- do_wait_par_thread loc p e t ;;cvm
+  i <- get_evid ;;cvm
+  sc <- get_config ;;cvm
+  rem_evs <- match events_fix (session_context sc) p (get_et e) t i with
+  | err e => CVM_fail (dispatch_error (Runtime e))
+  | res evs => CVM_ret evs
+  end ;;cvm
+  add_trace rem_evs ;;cvm
+  inc_par_event_ids e t ;;cvm
+  i <- inc_id ;;cvm
+  add_trace [cvm_thread_end i loc] ;;cvm
+  CVM_ret e'.
 Hint Unfold wait_par_thread : cvm.
 
 (* Some other hints relevant to CVM *)
