theories/St.v
@@ -45,6 +45,39 @@ Definition CVM_Error_to_string (e : CVM_Error) : string :=
     | Runtime s => "dispatch_error: " ++ s
     end
   end.
+Opaque CVM_Error_to_string.
 
 Definition CVM A : Type := 
   Config Session_Config (State cvm_st (Result A CVM_Error)).
+
+Global Create HintDb cvm.
+
+Definition CVM_bind {A B} (m : CVM A) (f : A -> CVM B) : CVM B :=
+  fun conf st => 
+    let '(a, st') := m conf st in
+    match a with
+    | res a => f a conf st'
+    | err e => ret (err e) st
+    end.
+
+Definition CVM_ret {A} (a : A) : CVM A :=
+  fun _ st => (res a, st).
+Definition CVM_fail {A} (e : CVM_Error) : CVM A :=
+  fun _ st => (err e, st).
+Definition CVM_ask : CVM Session_Config :=
+  fun conf st => (res conf, st).
+Definition CVM_put (st : cvm_st) : CVM unit :=
+  fun _ _ => (res tt, st).
+Definition CVM_get : CVM cvm_st :=
+  fun _ st => (res st, st).
+
+Global Hint Unfold CVM_bind CVM_ret CVM_ask CVM_put CVM_get CVM_fail : cvm.
+
+Notation "x <- m ;;cvm c" := (CVM_bind m (fun x => c))
+  (at level 61, m at next level, right associativity).
+Notation "' pat <- m ;;cvm c" :=
+  (CVM_bind m (fun x => match x with pat => c end))
+  (at level 61, pat pattern, m at next level, right associativity).
+Notation "e1 ;;cvm e2" := (_ <- e1 ;;cvm e2) (at level 61, right associativity).
+
+Ltac2 Notation "cvm_monad_unfold" := ux cvm ().
